### 7.13
(a)
$\neg P_1 \vee \neg P_2 ... \neg P_m \vee Q \ \ equivalent\ to$
$\neg(P_1 \land P_2 \land P_3\ ...\ \land P_m)\ \vee \ Q\ \ equivalent\ to$
$(P_1 \land P_2 \land P_3\ ... \ \land P_m) \rightarrow Q$

(b)
只要把所有带有$\neg$的文字放在左边，不带的放在右边
$\neg P_1 \vee \neg P_2 \vee \neg P_3 ... \neg P_m \vee Q_1 ...\vee Q_n$
将$Q_1\vee Q_2 ...\vee Q_n$视作整体，得
$(P_1 \land P_2 ... \land P_m)\rightarrow (Q_1 \vee Q_2 ...\vee Q_n)$

(c)
$假设p_n=s_1$
$$
\frac{p_1 \land p_2 ...\land p_m \rightarrow q_1\vee q_2...\vee q_n \newline r}{}
$$

