
### t2的计算
P1的ROBDD如下所示：

![|257](https://raw.githubusercontent.com/ustc21xyx/picture-bed/main/20240501144400.png)
$P2的ROBDD就是t1的ROBDD,将a_2修改为a_2'$
![](https://raw.githubusercontent.com/ustc21xyx/picture-bed/main/20240501145122.png)
故$t_{2}=\exists a_1',a_{2}' \ \ ROBDD(P1)\land ROBDD(P2)$ 


先计算$ROBDD(P)=ROBDD(P1)\land ROBDD(P2)$,所得ROBDD如下
![](https://raw.githubusercontent.com/ustc21xyx/picture-bed/main/20240501154648.png)

$再计算ROBDD(S_{p_e})=ROBDD(\exists a_{1}' a_{2}'\ \ P)$
![|257](https://raw.githubusercontent.com/ustc21xyx/picture-bed/main/20240501151617.png)
最后再计算$ROBDD(S_{p_{2}\land}T)，得$
![|195](https://raw.githubusercontent.com/ustc21xyx/picture-bed/main/20240501152252.png)


### t3的计算
P1的ROBDD不变
$P2的ROBDD就是t2的ROBDD,将a_{1}修改为a_{1}',a_2修改为a_2'$
![|109](https://raw.githubusercontent.com/ustc21xyx/picture-bed/main/20240501152737.png)
先计算$ROBDD(P)=ROBDD(P1)\land ROBDD(P2)$,所得ROBDD如下:
![|338](https://raw.githubusercontent.com/ustc21xyx/picture-bed/main/20240501160848.png)

$再计算ROBDD(S_{p_e})=ROBDD(\exists a_{1}' a_{2}'\ \ P),所得如下$
![|257](https://raw.githubusercontent.com/ustc21xyx/picture-bed/main/20240501151617.png)
最后再计算$ROBDD(S_{p_{2}\land}T)，得$
![|195](https://raw.githubusercontent.com/ustc21xyx/picture-bed/main/20240501152252.png)